Refactor 'make_run_next_sprint_avoids_blocked...'
The logic in the induction step of this proof is likely required for
other proofs also. Factor it out and generalize it into its own proof.
Specifically, this is the logic that shows a sprint can never reach a
far cell in the west wall and will never have a cell eaten by a nice
devil on some future step.

AngelDevil/Runner.lean
@@ -71,8 +71,10 @@ lemma final_state_loc_eq_journey_last {p : Nat} (S : RunBuilder p) :
     exact S.dest (List.ne_nil_of_length_pos (Nat.pos_of_ne_zero hlz))
 
 -- List of cells necessary to prevent the runner from ever moving west of the y-axis
+-- TODO: Reevaluate whether the size of the wall should be smaller by 'p'
+-- I increased it to make sure one of the proofs would work but it may not be necessary.
 def west_wall (p n : Nat) :=
-  List.map (fun i : Nat ↦ (-1, (i : Int))) (List.range (p * n + 1))
+  List.map (fun i : Nat ↦ (-1, (i : Int))) (List.range (p * (n + 1) + 1))
 
 -- Any cell which is an elment of the west wall has x-coordinate -1
 lemma west_wall_xcoord_of_mem (p n : Nat) :
@@ -85,7 +87,7 @@ lemma west_wall_xcoord_of_mem (p n : Nat) :
 
 -- Prove the conditions for a cell to be an element of the west wall
 lemma west_wall_mem (p n : Nat) :
-  ∀ i (_ : i ≤ p * n), (-1, Int.ofNat i) ∈ west_wall p n := by
+  ∀ i (_ : i ≤ p * (n + 1)), (-1, Int.ofNat i) ∈ west_wall p n := by
   intro i ile
   unfold west_wall
   apply List.mem_iff_getElem.mpr
@@ -538,6 +540,26 @@ lemma make_run_sprint_mem_journey_cell_close (D : Devil) (p n : Nat) :
   · convert hmem
     exact Nat.sub_one_add_one inz
 
+-- Every element of the 'next_sprint' is close to the previous journey cell
+lemma make_run_next_sprint_mem_journey_cell_close (D : Devil) (p n : Nat) :
+  ∀ rs ∈ next_sprint (make_run D p n),
+  close p (loc rs) (cell (make_run D p n).A n (by
+    rw [make_run_journey_steps]; exact Nat.lt_add_one _)
+  ) := by
+  intro rs rsmem
+  have rsmem' : rs ∈ (make_run D p (n + 1)).sprints[n]'(by
+    rw [make_run_sprints_length]; exact Nat.lt_add_one _
+  ) := by
+    rw [getElem_congr_coll (make_run_sprints_recurrence D p (n + 1) (Nat.add_one_pos _))]
+    rw [List.getElem_append_right]; swap
+    · rw [make_run_sprints_length, Nat.add_one_sub_one]
+    rw [List.getElem_singleton]
+    rwa [Nat.add_one_sub_one]
+  convert make_run_sprint_mem_journey_cell_close D p (n + 1) n (Nat.lt_add_one _) rs rsmem' using 1
+  have mrsj := make_run_subjourney D p n (n + 1) (lt_trans (Nat.lt_add_one _) (Nat.lt_add_one _))
+  rw [← cell_congr_journey mrsj, subjourney_cell]
+  exact le_refl _
+
 -- List of blocked cells used to generate 'next_sprint (make_run D p n)'
 def make_block_list (D : Devil) (p n : Nat) : List (Int × Int) :=
   List.union (make_run D p n).eaten (west_wall p (make_run D p n).eaten.length)
@@ -546,6 +568,103 @@ def make_block_list (D : Devil) (p n : Nat) : List (Int × Int) :=
 lemma next_sprint_make_run_def (D : Devil) (p n : Nat) :
   next_sprint (make_run D p n) =
   sprint p (final_state (make_run D p n)) (make_block_list D p n) := rfl
+
+-- The final state of a 'make_run' is a member of the 'next_sprint' of a smaller make_run
+lemma make_run_final_state_mem_next_state (D : Devil) (p n : Nat) (npos : 0 < n) :
+(final_state (make_run D p n)) ∈ next_sprint (make_run D p (n - 1)) := by
+  have hsnnil : (make_run D p n).sprints ≠ [] := by
+    apply List.ne_nil_of_length_pos
+    rwa [make_run_sprints_length]
+  convert final_state_getLast_mem_of_nonnil (make_run D p n) hsnnil
+  rw [List.getLast_congr _ _ (make_run_sprints_recurrence D p n npos)]; swap
+  · apply List.append_ne_nil_of_right_ne_nil
+    exact list_singleton_ne_nil _
+  rw [List.getLast_append_right]; swap
+  · exact list_singleton_ne_nil _
+  rw [List.getLast_singleton]
+
+-- This theorem is a bit odd, but useful in several places.
+-- It states that a 'make_run' never steps on a later block list, given
+-- that it never steps on its own block list and the devil is nice.
+-- In some sense, this is the induction step for the more general
+-- 'make_run_next_sprint_avoids_blocked_of_nice' (see below).
+lemma make_run_next_sprint_avoids_later_block_list_of_nice
+  (D : Devil) (p n : Nat) (hnice : nice D p) :
+  ∀ rs ∈ next_sprint (make_run D p n), loc rs ∉ make_block_list D p n →
+  ∀ n' (_ : n ≤ n'), loc rs ∉ make_block_list D p n' := by
+  intro rs rsmemns rsnmembl n' nle rsmembl'
+  have nnen' : n ≠ n' := by
+    intro nn'
+    subst nn'
+    exact rsnmembl rsmembl'
+  have nltn' : n < n' := Nat.lt_of_le_of_ne nle nnen'
+  by_cases n'z : n' = 0
+  · subst n'z
+    exact nnen' (Nat.le_zero.mp nle)
+  rename' n'z => n'nz; push_neg at n'nz
+  have n'pos : 0 < n' := Nat.pos_of_ne_zero n'nz
+  rcases List.mem_union_iff.mp rsmembl' with lhs | rhs
+  · -- Handle the case where the 'rs' is on the eaten list
+    rcases List.getElem_of_mem lhs with ⟨i, ilt, hi⟩
+    rw [make_run_eaten_length] at ilt
+    rw [make_run_eaten D p n' i ilt] at hi
+    -- Handle the case where 'rs'  was eaten after it was visited
+    by_cases nlt : n < i
+    · -- Since 'rs' is in the previous sprint, the devil has eaten a cell
+      -- close to a previous journey cell, which contradicts 'hnice'.
+      apply not_nice_of_eats_close D p _ hnice
+      use (make_run D p n').A, n, i, nlt
+      use (by rwa [make_run_journey_steps])
+      rw [make_run_subjourney, hi, close_comm]; swap
+      · exact ilt
+      apply make_run_sprint_mem_journey_cell_close; swap
+      · exact nltn'
+      rw [make_run_sprint]
+      · exact rsmemns
+      · exact nltn'
+    · rename' nlt => ile; push_neg at ile
+      -- If i ≤ n, we will show that 'rs' was on the old eaten list - a contradiction
+      apply rsnmembl
+      apply List.mem_union_iff.mpr; left
+      rw [← hi]
+      have ilt' : i < (make_run D p n).eaten.length := by
+        rw [make_run_eaten_length]
+        exact Nat.lt_add_one_of_le ile
+      convert List.getElem_mem ilt'; symm
+      exact make_run_eaten D p n i (Nat.lt_add_one_of_le ile)
+  -- Now handle the case where 'rs' is a wall cell
+  · unfold west_wall at rhs
+    rcases List.getElem_of_mem rhs with ⟨i, ilt, hi⟩
+    rw [List.length_map, List.length_range, make_run_eaten_length] at ilt
+    rw [List.getElem_map, List.getElem_range] at hi
+    -- Handle the case where 'i' is so large, it exceeds the bound proven in Bound.lean
+    by_cases lti : p * (n + 1) < i
+    · have hclose₀ : close (p * n) (0, 0) (last (make_run D p n).A) := by
+        unfold close
+        by_contra! h
+        apply (lt_self_iff_false n).mp
+        nth_rw 2 [← make_run_journey_steps D p n]
+        exact journey_lb _ _ h
+      have hclose₁ : close p (last (make_run D p n).A) (loc rs) := by
+        rw [close_comm, last]
+        rw [cell_congr_idx (make_run D p n).A (make_run_journey_steps D p n)]
+        apply make_run_next_sprint_mem_journey_cell_close
+        assumption
+      have hclose₂ : close (p * (n + 1)) (0, 0) (loc rs) := by
+        rw [mul_add, mul_one]
+        exact le_trans (dist_tri _ _ _) (Nat.add_le_add hclose₀ hclose₁)
+      apply not_lt_of_ge (close_origin_yle _ _ hclose₂)
+      rw [← hi]; simp
+      rwa [← Int.ofNat_one, ← Int.natCast_add, Int.ofNat_mul_ofNat, Int.ofNat_lt]
+    rename' lti => ile; push_neg at ile
+    · -- If i ≤ p * (n + 1), show that 'rs' was in the old west wall
+      apply rsnmembl (List.mem_union_iff.mpr _); right
+      rw [make_run_eaten_length, ← hi]
+      apply west_wall_mem
+      -- TODO: We have some slack here, which suggests that
+      -- one of our definitions isn't as tight as it should be
+      rw [mul_add]
+      exact Nat.le_add_right_of_le ile
 
 /- Note that it *is* possible to force the runner to remain on a blocked cell
    if the devil is not nice. Technically, even with a devil that isn't nice,
@@ -595,65 +714,11 @@ lemma make_run_next_sprint_avoids_blocked_of_nice (D : Devil) (p n : Nat) (hnice
       exact list_singleton_ne_nil _
     rw [List.getLast_append_right (list_singleton_ne_nil _)]
     exact (List.getLast_singleton (list_singleton_ne_nil _)).symm
-  -- Strengthen the statement of 'hsafe' by including the devil's last response and
-  -- an extra 'p' cells in the west wall. This section constitutes the majority of the proof.
-  have hsafe' : loc (final_state (make_run D p n)) ∉ make_block_list D p n := by
-    intro lfsmem
-    rcases List.mem_union_iff.mp lfsmem with lhs | rhs
-    · -- Handle the case where the final state is on the 'eaten' list
-      rcases List.getElem_of_mem lhs with ⟨i, ilt, hi⟩
-      rw [make_run_eaten_length] at ilt
-      rw [getElem_congr_coll (make_run_eaten_recurrence D p n (Nat.pos_of_ne_zero nnz))] at hi
-      -- Handle the case where the final state was eaten last
-      by_cases hin : i = n
-      · rw [List.getElem_append_right] at hi; swap
-        · rw [make_run_eaten_length, hin, Nat.sub_one_add_one nnz]
-        -- Prove a bound needed for 'getElem_singleton'
-        have lt1 : i - (make_run D p (n - 1)).eaten.length < 1 := by
-          rw [make_run_eaten_length, Nat.sub_one_add_one nnz, hin, Nat.sub_self]
-          norm_num
-        rw [List.getElem_singleton lt1, final_state_loc_eq_journey_last] at hi
-        -- We will show that a journey cell is eaten, which is contradiction with 'hnice'
-        apply not_nice_of_eats_journey_cell D p _ hnice
-        use (make_run D p n).A, n, n, le_refl n
-        use (by rw [make_run_journey_steps]; exact Nat.lt_add_one _)
-        have hsj := subjourney_full (make_run D p n).A
-        rw [subjourney_congr_idx _ (make_run_journey_steps D p n)] at hsj
-        rw [hsj]
-        convert hi
-        rw [last]
-        congr
-        rw [make_run_journey_steps]
-      · rename' hin => inen; push_neg at inen
-        -- If i ≠ n, we will show that the final state was on the old eaten list - a contradiction
-        apply hsafe
-        apply List.mem_union_iff.mpr; left
-        have ilt' : i < (make_run D p (n - 1)).eaten.length := by
-          rw [make_run_eaten_length, Nat.sub_one_add_one nnz]
-          exact lt_of_le_of_ne (Nat.le_of_lt_add_one ilt) inen
-        rw [List.getElem_append_left ilt'] at hi
-        exact List.mem_of_getElem hi
-    · -- Now handle the case where the final state is a wall cell
-      unfold west_wall at rhs
-      rcases List.getElem_of_mem rhs with ⟨i, ilt, hi⟩
-      rw [List.length_map, List.length_range, make_run_eaten_length] at ilt
-      rw [List.getElem_map, final_state_loc_eq_journey_last] at hi
-      -- Handle the case where 'i' is so large, it exceeds the bound proven in Bound.lean
-      by_cases pni : p * n < i
-      · apply (lt_self_iff_false n).mp
-        nth_rw 2 [← make_run_journey_steps D p n]
-        apply journey_lb _ _ (lt_of_lt_of_le pni (le_trans _ (le_max_right _ _)))
-        simp
-        rw [← (Prod.ext_iff.mp hi).2, List.getElem_range]
-        exact (le_refl i)
-      rename' pni => ilepn; push_neg at ilepn
-      · -- If i ≤ p * n, show that the final state was in the old west wall
-        apply hsafe (List.mem_union_iff.mpr _); right
-        rw [List.getElem_range] at hi
-        rw [final_state_loc_eq_journey_last, ← hi]
-        apply west_wall_mem
-        rwa [make_run_eaten_length, Nat.sub_one_add_one nnz]
-  exact sprint_avoids_blocked p _ _ hsafe' rs rsmem lrsmem
+  have fsmem := make_run_final_state_mem_next_state D p n (Nat.pos_of_ne_zero nnz)
+  -- The induction step for our argument was proven separately: showing that any cell in
+  -- 'next_sprint' that isn't in its own block list won't be in any future block list.
+  have := make_run_next_sprint_avoids_later_block_list_of_nice D p (n - 1) hnice _ fsmem hsafe n (Nat.sub_le _ _)
+  exact sprint_avoids_blocked p _ _ this rs rsmem lrsmem
 
 lemma make_run_journey_allowed_of_nice (D : Devil) (p n : Nat) (hnice : nice D p) :
   allowed D (make_run D p n).A := by
